Verse/Arch.v
@@ -1,9 +1,11 @@
 Require Import Verse.Language.
 Require Import Verse.Syntax.
+Require Import Verse.Function.
 Require Import Verse.Types.Internal.
 Require Import String.
 Require Import List.
 Import ListNotations.
+Require Import Basics.
 
 Module Type ARCH.
 
@@ -15,14 +17,6 @@ Module Type ARCH.
 
   Parameter reg : varT.
   Parameter stack : varT.
-
-  (* #####################
-     The archvar to be passed to functions would be something like this
-  *)
-  Inductive farchvar : varT :=
-  | rv (ty : type) : reg ty -> farchvar ty
-  | sv (ty : type) : farchvar ty
-  .
 
   Inductive var  : varT :=
   | r (ty : type)  : reg ty -> var ty
@@ -39,37 +33,18 @@ Module Type ARCH.
     | i :: bt => and (wfinstr i) (wfinstrB bt)
     end.
 
+
+  Parameter callConv : forall {p l : list type}, betaT var (p ++ l).
+
+  Definition alloc (p lv lr : list type) (t : type) (lalloc : @betaT reg lr) (f : function p lv lr t) : FB var t :=
+    (lalloc _) (lam_cv r (callConv _ ((tr f) var))).
+ 
+
   (** Generate code with assurance of well formedness **)
-
-  (* #####################
-     Could have a notation for @sigT type and projT1 
-  *)
-
-  Parameter callConv : forall lt, {lv : list (sigT farchvar) | map (@projT1 _ farchvar) lv = lt}.
-
-  (* #####################
-     The following would be the stack allocator that computes offsets 
-     given the complete allocation 'list'. However I cannot think of 
-     what proof obligation I want the function to satisfy.
-  *)
-  Parameter stalloc  : forall (l : list (sigT farchvar)), list (sigT var).
-
   Parameter generate : forall b : block var, wftypesB b -> wfvarB b -> wfinstrB b -> string.
   
-  (**
-
-    Translate the assignment statement to assembly. Certain assignment
-    instructions can fail, for example a three address assignment like
-    [A <= B + C] is not supported on a 2-address machine like x86. and
-    hence the result of a translation is a [option (list mnemonic)]
-    instead of just a [list mnemonics].
-
-   *)
-
-  (** Convert the loop statement in assembly instruction. *)
-  (*Parameter loop
-  : forall {b : bound}{ty : type (Bounded b)},
-      var reg ty -> arg reg ty -> list mnemonic -> list mnemonic.*)
-
 End ARCH.
 
+
+
+  
